theories/models/utp_vdm_simple/utp_vdm_types.thy
@@ -61,7 +61,7 @@ done
 definition InvS :: "'a set \<Rightarrow> ('a \<Rightarrow> bool vdme) \<Rightarrow> 'a set" where
 "InvS A P = {x. x \<in> A \<and> (\<forall> b. \<lbrakk>P x\<rbrakk>\<^sub>* b = Some True)}"
 
-nonterminal vty
+declare InvS_def [eval,evale,evalp]
 
 syntax 
   "_vty_quote"   :: "string \<Rightarrow> vty" ("<_>")
@@ -79,7 +79,7 @@ syntax
   "_vty_seq_of"  :: "vty \<Rightarrow> vty" ("@seq of _")
   "_vty_seq1_of" :: "vty \<Rightarrow> vty" ("@seq1 of _")
   "_vty_prod"    :: "vty \<Rightarrow> vty \<Rightarrow> vty" (infixl "\<times>" 20)
-  "_vty_quo"     :: "vty \<Rightarrow> 'a set" ("\<parallel>_\<parallel>")
+  "_vty_quo"     :: "vty \<Rightarrow> 'a set" ("\<parallel>_\<parallel>\<^sub>t")
   "_vty_inv"     :: "vty \<Rightarrow> pttrn \<Rightarrow> pexpr \<Rightarrow> vty" ("_ inv _ == _")
 
 translations
@@ -101,8 +101,10 @@ translations
   "_vty_quo x"     => "x"
   "_vty_inv A x P" == "CONST InvS A (\<lambda>x. P)"
 
-term "\<parallel>@seq1 of @char\<parallel>"
+term "\<parallel>@seq1 of @char\<parallel>\<^sub>t"
 
 (* term "`x := \<langle><1>\<rangle> : @seq1 of @nat1`" *)
+
+term "\<parallel>[\<langle>1\<rangle>] : @seq1 of @int\<parallel>"
 
 end
